ProtoQuipperFormalization/README.md
@@ -4,14 +4,4 @@ By Mohamed Yousri Mahmoud and Amy P. Felty
 
 Home: https://www.site.uottawa.ca/~afelty/jar19/
 
-## Building
-Only works up to Coq 8.10.2.
-
-First time setup to get the right version of Coq:
-```bash
-opam switch create 4.09.1
-eval $(opam env)
-opam pin add coq 8.10.2
-```
-
-Then the usual `make`.
+Updated to work with recent versions of Hybrid library and Coq v8.13.2.
